TheoryTask/qcp-binary-democases/SeparationLogic/examples/sll_project_strategy_goal.v
@@ -95,23 +95,6 @@ Definition sll_project_strategy14 :=
     ((sllseg p p l))
     ).
 
-Definition sll_project_strategy15 :=
-  forall (l : (@list Z)) (p : Z),
-    TT &&
-    emp **
-    ((sllseg p p l))
-    |--
-    (
-    TT &&
-    ([| (l = (@nil Z)) |]) &&
-    emp
-    ) ** (
-    TT &&
-    emp -*
-    TT &&
-    emp
-    ).
-
 Definition sll_project_strategy31 :=
   forall (p : Z),
     TT &&
@@ -144,23 +127,6 @@ Definition sll_project_strategy20 :=
     TT &&
     emp **
     ((sllbseg p p l))
-    ).
-
-Definition sll_project_strategy21 :=
-  forall (l : (@list Z)) (p : Z),
-    TT &&
-    emp **
-    ((sllbseg p p l))
-    |--
-    (
-    TT &&
-    ([| (l = (@nil Z)) |]) &&
-    emp
-    ) ** (
-    TT &&
-    emp -*
-    TT &&
-    emp
     ).
 
 Definition sll_project_strategy40 :=
@@ -294,27 +260,6 @@ Definition sll_project_strategy61 :=
     ([| (x1 = x2) |]) &&
     ([| (l1 = l2) |]) &&
     emp
-    ) ** (
-    TT &&
-    emp -*
-    TT &&
-    emp
-    ).
-
-Definition sll_project_strategy34 :=
-  forall (p : Z) (pt : Z) (h : Z) (l : (@list Z)),
-    TT &&
-    ([| (p <> 0) |] || [| (0 <> p) |]) &&
-    emp **
-    ((poly_store FET_ptr &( ((p)) # "sllb" ->ₛ "head") h)) **
-    ((poly_store FET_ptr &( ((p)) # "sllb" ->ₛ "ptail") pt)) **
-    ((sll h l))
-    |--
-    (
-    TT &&
-    ([| (p <> 0) |] || [| (0 <> p) |]) &&
-    emp **
-    ((sllb p l))
     ) ** (
     TT &&
     emp -*
@@ -682,24 +627,6 @@ Definition sll_project_strategy71 :=
     emp
     ).
 
-Definition sll_project_strategy89 :=
-  forall (y : Z) (v : Z) (z : Z) (p : Z),
-    TT &&
-    emp **
-    ((UIntArray.ceil_shape p y z)) **
-    ((poly_store FET_uint (Z.add p (Z.mul z (@sizeof_front_end_type FET_uint))) v))
-    |--
-    (
-    TT &&
-    emp **
-    ((UIntArray.ceil_shape p y (Z.add z 1)))
-    ) ** (
-    TT &&
-    emp -*
-    TT &&
-    emp
-    ).
-
 Definition sll_project_strategy32 :=
   forall (p : Z) (l : (@list Z)),
     TT &&
@@ -720,26 +647,6 @@ Definition sll_project_strategy32 :=
       TT &&
       emp
       ).
-
-Definition sll_project_strategy33 :=
-  TT &&
-  emp
-  |--
-  (
-  TT &&
-  emp
-  ) ** (
-  ALL (p : Z) (pt : Z) (h : Z) (l : (@list Z)),
-    TT &&
-    ([| (p <> 0) |]) &&
-    emp **
-    ((poly_store FET_ptr &( ((p)) # "sllb" ->ₛ "head") h)) **
-    ((poly_store FET_ptr &( ((p)) # "sllb" ->ₛ "ptail") pt)) **
-    ((sll h l)) -*
-    TT &&
-    emp **
-    ((sllb p l))
-    ).
 
 Definition sll_project_strategy70 :=
   forall (i : Z) (n : Z) (p : Z),
@@ -768,10 +675,8 @@ Module Type sll_project_Strategy_Correct.
   Axiom sll_project_strategy5_correctness : sll_project_strategy5.
   Axiom sll_project_strategy6_correctness : sll_project_strategy6.
   Axiom sll_project_strategy14_correctness : sll_project_strategy14.
-  Axiom sll_project_strategy15_correctness : sll_project_strategy15.
   Axiom sll_project_strategy31_correctness : sll_project_strategy31.
   Axiom sll_project_strategy20_correctness : sll_project_strategy20.
-  Axiom sll_project_strategy21_correctness : sll_project_strategy21.
   Axiom sll_project_strategy40_correctness : sll_project_strategy40.
   Axiom sll_project_strategy41_correctness : sll_project_strategy41.
   Axiom sll_project_strategy42_correctness : sll_project_strategy42.
@@ -780,7 +685,6 @@ Module Type sll_project_Strategy_Correct.
   Axiom sll_project_strategy52_correctness : sll_project_strategy52.
   Axiom sll_project_strategy60_correctness : sll_project_strategy60.
   Axiom sll_project_strategy61_correctness : sll_project_strategy61.
-  Axiom sll_project_strategy34_correctness : sll_project_strategy34.
   Axiom sll_project_strategy7_correctness : sll_project_strategy7.
   Axiom sll_project_strategy16_correctness : sll_project_strategy16.
   Axiom sll_project_strategy30_correctness : sll_project_strategy30.
@@ -801,9 +705,7 @@ Module Type sll_project_Strategy_Correct.
   Axiom sll_project_strategy92_correctness : sll_project_strategy92.
   Axiom sll_project_strategy93_correctness : sll_project_strategy93.
   Axiom sll_project_strategy71_correctness : sll_project_strategy71.
-  Axiom sll_project_strategy89_correctness : sll_project_strategy89.
   Axiom sll_project_strategy32_correctness : sll_project_strategy32.
-  Axiom sll_project_strategy33_correctness : sll_project_strategy33.
   Axiom sll_project_strategy70_correctness : sll_project_strategy70.
 
 End sll_project_Strategy_Correct.
